theories/PCP/MPCP_BMPCP.v
@@ -1,0 +1,111 @@
+Require Import ssreflect ssrbool ssrfun.
+Require Import List.
+Import ListNotations.
+
+From Undecidability Require Import Problems.PCP Problems.Reduction.
+
+(* map a n-ary string to a binary string *)
+Definition bin (x: list nat) : list bool := flat_map (fun (a : nat) => true :: (repeat false a) ++ [true])  x.
+
+Lemma eq_binP {x y} : x = y <-> (bin x) = (bin y).
+Proof.
+  elim: x y.
+    by case.
+  move=> a x IH. case.
+    done.
+  move=> b y /=. constructor.
+    by case=> <- <-.
+  case. elim: a b.
+    case=> /=.
+      case. by move /IH => ->.
+    done.
+  move=> a IH2. case=> /=.
+    done.
+  move=> b. case=> /IH2. by case=> <- <-.
+Qed.
+
+Lemma bin_appP {x y} : bin (x ++ y) = bin x ++ bin y.
+Proof. 
+  by rewrite /bin ? flat_map_concat_map map_app concat_app.
+Qed.
+
+Definition bin_map A := map (fun '(x, y) => (bin x, bin y)) A.
+
+Lemma map_consP {X Y: Type} {f: X -> Y} {a: X} {A : list X}: map f (a :: A) = (f a) :: map f A.
+Proof. done. Qed.
+
+Lemma tau1_bin_map {A : list (list nat * list nat)} : tau1 (bin_map A) = bin (tau1 A).
+Proof.
+  elim: A.
+    done.
+  move=> [x y] A IH.
+  rewrite /bin_map map_consP /tau1 -/tau1 bin_appP. 
+  by f_equal.
+Qed.
+
+Lemma tau2_bin_map {A : list (list nat * list nat)} : tau2 (bin_map A) = bin (tau2 A).
+Proof.
+  elim: A.
+    done.
+  move=> [x y] A IH.
+  rewrite /bin_map map_consP /tau2 -/tau2 bin_appP. 
+  by f_equal.
+Qed.
+
+Lemma Forall_consP {T: Type} {P : T -> Prop} {a: T} {l: list T} :
+  Forall P (a :: l) <-> P a /\ Forall P l.
+Proof.
+  constructor. 
+    move=> H. by inversion H.
+  move=> [? ?]. by constructor.
+Qed.
+
+Lemma incl_consP {X: Type} {a: X} {A: list X} {P: list X} : (incl (a :: A) P) <-> (In a P /\ incl A P).
+Proof.
+  by rewrite /incl - ? Forall_forall Forall_consP. 
+Qed.
+
+(* preimage of a mapped list  *)
+Lemma debin {A: list (list bool * list bool)} {P : list (list nat * list nat)} : 
+  incl A (bin_map P) -> exists B, A = bin_map B /\ incl B P.
+Proof.
+  elim: A.
+    move=> *. exists []. by constructor.
+  move=> a A IH /incl_consP [+ +].
+  rewrite /bin_map. move /(@in_map_iff) => [[x' y'] [? ?]]. subst a.
+  move /IH => [B [? ?]]. exists ((x', y') :: B). constructor.
+    by subst A.
+  apply /incl_consP. by constructor.
+Qed.
+
+From Undecidability Require Import PCP.Definitions.
+
+(* 
+  many-one reduction from the modified Post correspondence problem 
+  to the binary modified Post correspondence problem
+*)
+Theorem MPCP_to_BMPCP : MPCP ⪯ BMPCP.
+Proof.
+  rewrite /reduces.
+  pose f := fun '((x, y), P) => ((bin x, bin y), bin_map P).
+  exists f.
+  move=> [[x y] P]. constructor.
+    move=> [A].
+    move=> [HA1 HA2].
+    exists (bin_map A).
+    constructor.
+      move=> a.
+      move /in_map_iff => [a' [?]] /HA1. subst a.
+      rewrite -/(map _ ((x, y) :: P)).
+      by move /(in_map (fun '(x, y) => (bin x, bin y))).
+    by rewrite tau1_bin_map tau2_bin_map - ? bin_appP - eq_binP.
+  move=> [A]. case.
+  rewrite /bin_map -/(map _ ((x, y) :: P)) -/(bin_map _).
+  move /debin => [B [? ?]]. subst A.
+  rewrite tau1_bin_map tau2_bin_map - ? bin_appP.
+  move /eq_binP => ?.
+  exists B. by constructor.
+Qed.
+
+Check MPCP_to_BMPCP.
+(* Print Assumptions MPCP_to_BMPCP. *)
