theories/Problems/LPB.v
@@ -1,0 +1,53 @@
+(* 
+  Autor(s):
+    Andrej Dudenhefner (1) 
+  Affiliation(s):
+    (1) Saarland Informatics Campus, Saarland University, Saarbrücken, Germany
+*)
+
+(* 
+  Problem:
+    Recognizing axiomatizations of in Hilber-style calculi (LPB)
+    (Linial-Post theorem, strengthened by Bokov [1,2])
+
+  LPB:
+    Given a list s₁,...,sₙ of formulae such that 
+    [a → b → a] ⊢ sᵢ is derivable for i = 1...n,
+    is [s₁,...,sₙ] ⊢ a → b → a derivable?
+  
+  References:
+    [1] Grigoriy V. Bokov: Undecidable problems for propositional calculi with implication. 
+      Logic Journal of the IGPL, 24(5):792–806, 2016. doi:10.1093/jigpal/jzw013
+    [2] Andrej Dudenhefner, Jakob Rehof: Lower End of the Linial-Post Spectrum. 
+      TYPES 2017: 2:1-2:15. doi: 10.4230/LIPIcs.TYPES.2017.2
+*)
+
+Require Import PeanoNat.
+Require Import List.
+Import ListNotations.
+
+(* propositional formulae s, t ::= a | s → t *)
+Inductive formula : Set :=
+  | var : nat -> formula
+  | arr : formula -> formula -> formula.
+
+(* the formula a → b → a *)
+Definition a_b_a : formula := arr (var 0) (arr (var 1) (var 0)).
+
+(* substitute ζ t replaces each variable n in t by ζ n *)
+Fixpoint substitute (ζ: nat -> formula) (t: formula) : formula :=
+  match t with
+  | var n => ζ n
+  | arr s t => arr (substitute ζ s) (substitute ζ t)
+  end.
+
+(* Hilbert-style calculus *)
+Inductive hsc (Gamma: list formula) : formula -> Prop :=
+  | hsc_var : forall (ζ: nat -> formula) (t: formula), In t Gamma -> hsc Gamma (substitute ζ t)
+  | hsc_arr : forall (s t : formula), hsc Gamma (arr s t) -> hsc Gamma s -> hsc Gamma t.
+
+(* list of formulae derivable from a → b → a *)
+Definition LPB_PROBLEM := { Gamma: list formula | forall s, In s Gamma -> hsc [a_b_a] s}.
+
+(* is the formula a → b → a derivable? *)
+Definition LPB (l : LPB_PROBLEM) := hsc (proj1_sig l) a_b_a.
